theories/AlmostStlc/SyntaxSeq.v
@@ -25,8 +25,12 @@ with comp : vtype -> ctx -> mfix_ctx -> Type :=
     comp t2 Γ MR
   | comp_call t1 t2 Γ MR R (xR : var R MR) (x : var (t1,t2) R) (v : value t1 Γ) : 
     comp t2 Γ MR
+  | comp_mfix t Γ MR R (bodies : mfix_bodies Γ (R :: MR) R) (c : comp t Γ (R :: MR)) :
+    comp t Γ MR
+  (*
   | comp_mfix t Γ MR R (xR : var R MR) (bodies : mfix_bodies Γ MR R) (c : comp t Γ MR) : 
     comp t Γ (remove R MR xR)
+  *)
   | comp_lift t Γ MR1 MR2 (c : comp t Γ MR2) : comp t Γ (MR1 ++ MR2)
   | comp_perm t Γ MR1 MR2 (Hperm : perm MR1 MR2) (e : comp t Γ MR1) :
     comp t Γ MR2
@@ -54,7 +58,7 @@ Arguments comp_match_list {_ _ _ _}.
 Arguments comp_split {_ _ _ _ _}.
 Arguments comp_app {_ _ _ _}.
 Arguments comp_call {_ _ _ _ _}.
-Arguments comp_mfix {_ _ _ _}.
+Arguments comp_mfix {_ _ _}.
 Arguments comp_lift {_ _ _ _}.
 Arguments comp_perm {_ _ _ _}.
 Arguments mfix_bodies_nil {_ _}.
