theories/AlmostStlc/TypesEquiv.v
@@ -35,12 +35,12 @@ where mfix_pre_equiv (MR : mfix_ctx) :
   mfix_pre_equiv (cons cf MR) :=
     sum_rel (call_frame_pre_equiv cf) (mfix_pre_equiv MR);
 }
-where call_frame_pre_equiv (cf : call_frame) :
-  Rel (denote_call_frame cf) (denote_call_frame cf) := 
+where call_frame_pre_equiv (R : call_frame) :
+  Rel (denote_call_frame R) (denote_call_frame R) := 
 {
   call_frame_pre_equiv nil := fun _ _ => False;
-  call_frame_pre_equiv (cons (t1,t2) cf') :=
-    sum_rel (types_equiv t1) (call_frame_pre_equiv cf')
+  call_frame_pre_equiv (cons (t1,t2) R) :=
+    sum_rel (types_equiv t1) (call_frame_pre_equiv R)
 }
 where mfix_post_equiv (MR : mfix_ctx) : 
   PostRel (denote_mrec_ctx (denote_mfix_ctx MR)) (denote_mrec_ctx (denote_mfix_ctx MR)) :=
@@ -48,12 +48,12 @@ where mfix_post_equiv (MR : mfix_ctx) :
   mfix_post_equiv nil := fun _ _ _ _ => False;
   mfix_post_equiv (cons cf MR) := SumPostRel (call_frame_post_equiv cf) (mfix_post_equiv MR);
 }
-where call_frame_post_equiv (cf : call_frame) : 
-  PostRel (denote_call_frame cf) (denote_call_frame cf) :=
+where call_frame_post_equiv (R : call_frame) : 
+  PostRel (denote_call_frame R) (denote_call_frame R) :=
 {
   call_frame_post_equiv nil := fun _ _ _ _ => False;
-  call_frame_post_equiv (cons (t1,t2) cf ) :=
-    SumPostRel (fun _ _ => types_equiv t2) (call_frame_post_equiv cf);
+  call_frame_post_equiv (cons (t1,t2) R) :=
+    SumPostRel (fun _ _ => types_equiv t2) (call_frame_post_equiv R);
 }.
 (* use to create relations for [Γ] -> mtree [MR] [t] *)
 
@@ -187,242 +187,16 @@ Proof.
 Qed.
 
 
-
-(*
-now show that for any d1 : denote MR, exists R t1 t2 xR x,
-  d1 = projT1 (call_mrec x xR v1)
-
-  then do these lemmas for insert rel
-
-Lemma mfix_pre_equiv_position_inv (MR : mfix_ctx) 
-      (d1 d2 : denote_mrec_ctx (denote_mfix_ctx MR)) :
-  mfix_pre_equiv MR d1 d2 ->
-  exists R (t1 t2 : type) (xR : var R MR) (x : var (t1,t2)),
-  d1 = projT1 (call_mrec x xR v1) ->
-  d2 = projT1 (call_mrec x xR v2) ->
-  types_equiv t1 v1 v2 ->
-  m.
+Lemma pre_equiv_sum_rel MR R : 
+  forall c1 c2, mfix_pre_equiv (R :: MR) c1 c2 <-> sum_rel (call_frame_pre_equiv R) (mfix_pre_equiv MR) c1 c2.
 Proof.
-() *)
-      (*
-InsertPreRel :
-forall {MR1 MR2 : mrec_ctx} {In1 In2 : Type} {Out1 : EncodedType In1} {Out2 : EncodedType In2} (x : var (In1 && Out1) MR1)
-  (y : var (In2 && Out2) MR2),
-Rel In1 In2 -> Rel (denote_remainder MR1 x) (denote_remainder MR2 y) -> Rel (denote_mrec_ctx MR1) (denote_mrec_ctx MR2)
+  rewrite mfix_pre_equiv_equation_2.
+  intros. reflexivity.
+Qed.
 
-mfix_pre_equiv
-     : forall MR : mfix_ctx, Rel (denote_mrec_ctx (denote_mfix_ctx MR)) (denote_mrec_ctx (denote_mfix_ctx MR))
-
-call_frame_pre_equiv
-     : forall cf : call_frame, Rel (denote_call_frame cf) (denote_call_frame cf)
-*)
-(*
-The term "mfix_pre_equiv (remove R MR xR)" has type
- "Rel (denote_mrec_ctx (denote_mfix_ctx (remove R MR xR))) (denote_mrec_ctx (denote_mfix_ctx (remove R MR xR)))"
-while it is expected to have type
- "Rel (denote_remainder (denote_mfix_ctx MR) (denote_var xR)) (denote_remainder (denote_mfix_ctx MR) (denote_var xR))"
-(cannot unify "denote_remainder (denote_mfix_ctx MR) (denote_var xR)" and "denote_mrec_ctx (denote_mfix_ctx (remove R MR xR))"
-
-need some kind of lift thing to commute
-
-*)
-
-
-(*
-Lemma insert_pre_rel_mfix_pre_equiv_aux1:
-  forall (a b : call_frame) (l : mfix_ctx) (xR : var a l)
-    (d : denote_mrec_ctx (denote_mfix_ctx' (List.map (List.map (fun '(t1, t2) => denote_type t1 && inout_encoded (denote_type t1) (denote_type t2))) l)))
-    (d0 : denote_mrec_ctx (denote_mfix_ctx' (List.map (List.map (fun '(t1, t2) => denote_type t1 && inout_encoded (denote_type t1) (denote_type t2))) l)))
-                 (a1 a2 : denote_call_frame a),
-    inl a2 = projT1 (bring_to_front (denote_mfix_ctx (b :: l)) (VarS (denote_var xR)) (inr d0)) ->
-    inl a1 = projT1 (bring_to_front (denote_mfix_ctx (b :: l)) (VarS (denote_var xR)) (inr d)) ->
-    call_frame_pre_equiv a a1 a2 ->
-    sum_rel (call_frame_pre_equiv a) (commute_remove_rel (mfix_pre_equiv (remove a l xR))) (projT1 (bring_to_front (denote_mfix_ctx l) (denote_var xR) d))
-            (projT1 (bring_to_front (denote_mfix_ctx l) (denote_var xR) d0)).
-Abort.
-
-Lemma insert_pre_rel_equiv_comp_equiv_aux2:
-  forall (a b : call_frame) (l : mfix_ctx) (xR : var a l) (x0 y : denote_mrec_ctx (denote_mfix_ctx (b :: l)))
-    (b1 b2 : denote_remainder (denote_mfix_ctx (b :: l)) (denote_var (VarS xR))),
-    commute_remove_rel (mfix_pre_equiv (remove a (b :: l) (VarS xR))) b1 b2 ->
-    (forall x y : denote_mrec_ctx (denote_mfix_ctx l),
-         InsertPreRel (denote_var xR) (denote_var xR) (call_frame_pre_equiv a) (commute_remove_rel (mfix_pre_equiv (remove a l xR))) x
-           y <-> mfix_pre_equiv l x y) ->
-    inr b1 = projT1 (bring_to_front (denote_mfix_ctx (b :: l)) (VarS (denote_var xR)) x0) ->
-    inr b2 = projT1 (bring_to_front (denote_mfix_ctx (b :: l)) (VarS (denote_var xR)) y) -> mfix_pre_equiv (b :: l) x0 y.
+Lemma post_equiv_sum_post_rel MR R : 
+  forall c1 c2 v1 v2, mfix_post_equiv (R :: MR) c1 c2 v1 v2 <-> SumPostRel (call_frame_post_equiv R) (mfix_post_equiv MR) c1 c2 v1 v2.
 Proof.
-  intros a b l xR x0 y b1 b2.
-  intros Hb12 IH Hb1 Hb2. red in Hb12. 
-  Transparent remove_denote. Transparent remove.
-  destruct (bring_to_front (denote_mfix_ctx (b :: l)) (VarS (denote_var xR)) x0) eqn : Heq1.
-  simpl in Hb1. subst.
-  destruct (bring_to_front (denote_mfix_ctx (b :: l)) (VarS (denote_var xR)) y) eqn : Heq2.
-  simpl in Hb2. subst.
-  simpl remove in Hb12. simpl in Hb12. 
-  dependent destruction Hb12.
-  - destruct b1; destruct b2.
-    * injection x1; injection x; intros; subst. clear x x1.
-      fold call_frame_pre_equiv in H.
-      destruct x0; destruct y.
-      -- constructor. fold call_frame_pre_equiv.
-         setoid_rewrite bring_to_front_equation_4 in Heq1.
-         setoid_rewrite bring_to_front_equation_4 in Heq2.
-         injection Heq1. intros. subst.
-         injection Heq2. intros. subst. auto.
-      -- setoid_rewrite bring_to_front_equation_5 in Heq2.
-         match goal with H : (let (x,f) := ?t in _ ) = _ |- _ =>
-                           destruct t as [ [? | ?] ? ]; discriminate end.
-      -- setoid_rewrite bring_to_front_equation_5 in Heq1.
-         match goal with H : (let (x,f) := ?t in _ ) = _ |- _ =>
-                           destruct t as [ [? | ?] ? ]; discriminate end.
-      -- constructor.
-         setoid_rewrite bring_to_front_equation_5 in Heq1.
-         match goal with H : (let (x,f) := ?t in _ ) = _ |- _ =>
-                           destruct t as [ [? | ?] ? ]; discriminate end.
-    * destruct (remove_denote xR d0); discriminate.
-    * destruct (remove_denote xR d); discriminate.
-    * destruct (remove_denote xR d); discriminate.
-  - destruct b1 eqn : Hb1'; try discriminate. destruct b2 eqn : Hb2'; try discriminate.
-    (**)
-    destruct x0; destruct y.
-    + constructor. fold call_frame_pre_equiv.
-      setoid_rewrite bring_to_front_equation_4 in Heq1. discriminate.
-    + setoid_rewrite bring_to_front_equation_4 in Heq1. discriminate.
-    + setoid_rewrite bring_to_front_equation_4 in Heq2. discriminate.
-    + setoid_rewrite bring_to_front_equation_5 in Heq1.
-      match goal with H : (let (x,f) := ?t in _ ) = _ |- _ =>
-                           destruct t as [ [? | ?] ? ] eqn : Heq3; try discriminate end.
-      injection Heq1. intros. subst. clear Heq1.
-      setoid_rewrite bring_to_front_equation_5 in Heq2.
-      match goal with H : (let (x,f) := ?t in _ ) = _ |- _ =>
-                           destruct t as [ [? | ?] ? ] eqn : Heq4; try discriminate end.
-      injection Heq2. intros. subst. clear Heq2.
-      constructor.
-      destruct (remove_denote xR d0) as [d0' ?] eqn : Heq5.
-      destruct (remove_denote xR d) as [d' ?] eqn : Heq6.
-      injection x. injection x1. intros. subst. clear x x1 IH.
-      (* possible that this case requires induction on xR 
-         
-
-       *)
-Abort. *)
-(* how would insert pre rel work with mfix pre rel 
-
-maybe consider using the position relation,
-if related, x and y must have the same position
-
-if they both have a position, then this relation reduces down 
-to the types equiv stuff, in any case call it for now
-
-*)
-
-(*
-       split.
-    + simpl denote_var. unfold InsertPreRel. 
-      intros. rewrite mfix_pre_equiv_equation_2.
-      simpl denote_mfix_ctx in H.
-      dependent destruction H.
-      * simp bring_to_front in x1.
-        simpl in x0, y.
-        destruct x0; destruct y; 
-        try setoid_rewrite bring_to_front_equation_2 in x1;
-        try setoid_rewrite bring_to_front_equation_2 in x;
-          try discriminate.
-        cbn in x, x1. injection x. injection x1. intros. subst.
-        constructor. auto.
-      * destruct x0; destruct y; 
-          try setoid_rewrite bring_to_front_equation_3 in x1;
-          try setoid_rewrite bring_to_front_equation_3 in x;
-          try discriminate.
-        injection x1. injection x. intros; subst.
-        constructor.
-        red in H.
-        assert (remove a (a :: l) VarZ  = l).
-        simp remove. auto.
-        setoid_rewrite remove_denote_equation_1 in H.
-        cbn in H.
-        clear - H. Transparent remove. cbn in H.
-        Opaque remove. auto.
-   + intros. rewrite mfix_pre_equiv_equation_2 in H.
-     red. dependent destruction H.
-     * constructor. auto.
-     * constructor. red.
-       setoid_rewrite remove_denote_equation_1.
-       Transparent remove. cbn. Opaque remove. auto.          
-  - split; intros.
-    + red in H. dependent destruction H.
-      * Transparent denote_var. simpl denote_var in x1, x.
-        destruct x0; destruct y;
-        try setoid_rewrite bring_to_front_equation_2 in x1;
-        try setoid_rewrite bring_to_front_equation_2 in x;
-          try discriminate.
-        constructor. apply IHxR. red.
-        eapply insert_pre_rel_mfix_pre_equiv_aux1; eauto.
-      * simpl denote_var in x, x1, H.
-        revert H x1 x.
-        red in H. admit.
-    + red in H. dependent destruction H. 
-      * do 2 constructor; auto.
-      * simpl denote_var. red. 
-        eapply IHxR in H. red in H.
-        dependent destruction H.
-        -- destruct 
-            ((bring_to_front (denote_mfix_ctx l) (denote_var xR) b1))
-            eqn : Heq1; cbn in x0; subst; try discriminate.
-          unfold denote_mfix_ctx. simpl.
-            rewrite bring_to_front_equation_5.
-            setoid_rewrite Heq1.
-            simpl.
-             destruct 
-            ((bring_to_front (denote_mfix_ctx l) (denote_var xR) b2))
-            eqn : Heq2; cbn in x; subst; try discriminate.
-          unfold denote_mfix_ctx. simpl.
-            rewrite bring_to_front_equation_5.
-            setoid_rewrite Heq2. constructor.
-            auto.
-       -- destruct 
-            ((bring_to_front (denote_mfix_ctx l) (denote_var xR) b1))
-            eqn : Heq1; cbn in x0; subst; try discriminate.
-          unfold denote_mfix_ctx. simpl.
-            rewrite bring_to_front_equation_5.
-            setoid_rewrite Heq1.
-            simpl.
-             destruct 
-            ((bring_to_front (denote_mfix_ctx l) (denote_var xR) b2))
-            eqn : Heq2; cbn in x; subst; try discriminate.
-          unfold denote_mfix_ctx. simpl.
-            rewrite bring_to_front_equation_5.
-            setoid_rewrite Heq2.
-            constructor.
-            clear - H. red. Transparent remove_denote.
-            red in H.
-            simpl remove_denote.
-            Transparent remove. simpl remove. simpl.
-            destruct (remove_denote xR b0);
-            destruct (remove_denote xR b3).
-            constructor. auto.
-Admitted. *)
-(* lets put this part aside for a bit and focus on another part *)
-(*
-Should be a PER 
-
-
-rewrite with eutt
-
-it should generalize eutt
-
-should be the case that if it is a denotation, then it is self related
-so it acts as an equivalence relation on its actual domain
-
-
-tomorrow would be a good time to get a basic sketch of rutt done at least,
-leave implementations of lemmas for later, there is a sense in which it is not
-along a critical path because it is known to be true, where as
-other things might actually include some bugs
-
-on monday work on this but also dedicate some time to the proposal intro
-
-
-also maybe go back to the comp_map proof and see what kind of reasoning principles are needed
-
-*)
+  rewrite mfix_post_equiv_equation_2.
+  intros. reflexivity.
+Qed.
