theories/Basics/Tactics.v
@@ -1,0 +1,6 @@
+Require Import Logic.Eqdep.
+
+Ltac inj_existT := 
+  repeat match goal with 
+         | H : existT _ _ _ = _ |- _ => apply inj_pair2 in H 
+         end.
