theories/Interp/Recursion.v
@@ -1,0 +1,34 @@
+Require Import ExtLib.Structures.Functor.
+Require Import ExtLib.Structures.Applicative.
+Require Import ExtLib.Structures.Monad.
+Require Import Program.Tactics.
+
+Require Import ITree.Basics.Basics.
+Require Import HeterogeneousRelations.
+
+Require Export EnTreeDefinition.
+Require Export SubEvent.
+
+
+Section interp_mrec.
+
+Context {D E : Type} `{enc1 : EncodedType D} `{enc2 : EncodedType E}.
+
+CoFixpoint interp_mrec' {R} (bodies : forall d : D, entree (D + E) (encodes d)) 
+           (ot : entree' (D + E) R) : entree E R :=
+  match ot with
+  | RetF r => Ret r
+  | TauF t => Tau (interp_mrec' bodies (observe t))
+  | VisF (inl d) k => Tau (interp_mrec' bodies (observe (bind (bodies d) k)))
+  | VisF (inr e) k => Vis e (fun x => interp_mrec' bodies (observe (k x)))
+  end.
+
+Definition interp_mrec {R} (bodies : forall d : D, entree (D + E) (encodes d)) 
+           (t : entree (D + E) R) : entree E R :=
+  interp_mrec' bodies (observe t).
+
+Definition mrec (bodies : forall d : D, entree (D + E) (encodes d))
+           (d : D) : entree E (encodes d) :=
+  interp_mrec bodies (trigger d).
+
+End interp_mrec. 
